add prop2.4

src/basic.lean
@@ -1,16 +1,34 @@
 import tactic
 
+open function set order
+
 -- Definition 2.1
 structure filter (X : Type*) :=
 (sets                     : set (set X))
 (upward_closure {F₁ F₂}   : F₁ ∈ sets → F₁ ⊆ F₂ → F₂ ∈ sets)
 (inter_sets {F₁ F₂}       : F₁ ∈ sets → F₂ ∈ sets → F₁ ∩ F₂ ∈ sets)
 
-instance {X : Type*} : has_mem (set X) (filter X) := ⟨λ U F, U ∈ F.sets⟩
-
 variables {X : Type*} {f g : filter X} {s : set X}
+namespace filter
 
-@[simp] lemma filter.mem_sets : s ∈ f.sets ↔ s ∈ f := iff.rfl
+instance : has_mem (set X) (filter X) := ⟨λ U F, U ∈ F.sets⟩
+
+@[simp] lemma mem_sets : s ∈ f.sets ↔ s ∈ f := iff.rfl
+
+lemma filter_eq : ∀ {f g : filter X}, f.sets = g.sets → f = g
+| ⟨a, _, _⟩ ⟨._, _, _⟩ rfl := rfl
+
+lemma filter_eq_iff : f = g ↔ f.sets = g.sets :=
+⟨congr_arg _, filter_eq⟩
+
+protected lemma ext_iff : f = g ↔ ∀ s, s ∈ f ↔ s ∈ g :=
+by simp only [filter_eq_iff, ext_iff, filter.mem_sets]
+
+@[ext]
+protected lemma ext : (∀ s, s ∈ f ↔ s ∈ g) → f = g :=
+filter.ext_iff.2
+
+end filter
 
 -- Definition 2.2
 structure filter_basis (X : Type*) :=
@@ -20,14 +38,22 @@ structure filter_basis (X : Type*) :=
 
 instance {X : Type*} : has_mem (set X) (filter_basis X) := sorry
 
-protected def filter_basis.filter (B : filter_basis X) : filter X :=
+-- Definition 2.2
+def filter_basis.filter (B : filter_basis X) : filter X :=
 { sets := {s | ∃ t ∈ B, t ⊆ s},
   upward_closure := sorry,
   inter_sets := sorry, }
 
+namespace filter
+
 -- Prop 2.3
-def filter.as_basis (f : filter X) : filter_basis X :=
+def as_basis (f : filter X) : filter_basis X :=
 ⟨f.sets, sorry⟩
 
 -- Prop 2.4
+lemma generated_filter_eq (h : filter_basis.filter (filter.as_basis f) = g) : 
+  f = g := sorry
+
+
+end filter
 
